theories/maps/linker/components/agree.v
@@ -1,0 +1,39 @@
+From main.prelude Require Import imports autosubst base_lang lists labels.
+From main.grad_lang Require Import types.
+From main.dyn_lang Require Import definition contexts lib casts.
+From main.maps Require Import grad_into_dyn.definition.
+From main.maps.linker.components Require Import dyn grd.
+
+Section agree.
+
+  Context {ν : label} {Hν : NeverOccurs ν}.
+
+  Lemma LamN_agree n e : ⌊ grd.LamN n e ⌋ = dyn.LamN n ⌊ e ⌋.
+  Proof. induction n; auto. simpl. by rewrite IHn. Qed.
+
+  Lemma LamN_ctx_agree n : trns_ctx $ grd.LamN_ctx n = dyn.LamN_ctx n.
+  Proof. induction n; auto. simpl. by rewrite IHn. Qed.
+
+  Lemma AppWithList_agree e fs :
+    ⌊ grd.AppWithList e fs ⌋ = dyn.AppWithList ⌊ e ⌋ ((fun f => ⌊ f ⌋) <$> fs).
+  Proof.
+    induction fs as [|f fs']; first auto.
+    rewrite /= /AppAn. f_equiv. by rewrite /IHfs'.
+  Qed.
+
+  Lemma AppWithList_ctx_agree ts :
+    trns_ctx $ grd.AppWithList_ctx ts = dyn.AppWithList_ctx (trns <$> ts).
+  Proof.
+    induction ts as [|t ts']; first auto.
+    rewrite /=. f_equiv. by rewrite IHts'.
+  Qed.
+
+  Lemma wrap_ctx_vars_ascribe_up_agree (ℓ : label) (Γ : list type) :
+    trns <$> (grd.wrap_ctx_vars_ascribe_up ℓ Γ) = dyn.wrap_ctx_vars_ascribe_up ℓ Γ.
+  Proof.
+    rewrite /grd.wrap_ctx_vars_ascribe_up /dyn.wrap_ctx_vars_ascribe_up.
+    rewrite fmap_imap. apply imap_ext. intros. simpl. rewrite /cast'.
+    destruct (consistency_decision x Unknown); auto.
+  Qed.
+
+End agree.
