theories/maps/linker/components/common.v
@@ -1,0 +1,9 @@
+From main.prelude Require Import imports base_lang.
+From main.grad_lang Require Import types.
+
+Definition LamN_type (Γ : list type) τ : type :=
+  foldl (fun T t => Bin Arrow t T) τ Γ.
+
+Definition LamN_type_snoc (Γ : list type) τ' τ :
+  LamN_type (Γ ++ [τ']) τ = (Bin Arrow τ' (LamN_type Γ τ)).
+Proof. by rewrite /LamN_type foldl_snoc. Qed.
