theories/maps/linker/definition.v
@@ -1,6 +1,6 @@
 From main.prelude Require Import imports labels.
 From main.grad_lang Require Import definition types typing contexts.
-From main.maps Require Import linker.components.
+From main.maps.linker.components Require Import common dyn grd.
 
 (* Notation gexpr := grad_lang.definition.expr. *)
 (* Notation dexpr := dyn_lang.definition.expr. *)
@@ -8,8 +8,6 @@ From main.maps Require Import linker.components.
 (* Notation gApp := grad_lang.definition.Var. *)
 
 Section linker.
-
-  Context {ν : label} {Hν : NeverOccurs ν}.
 
   (* todo; generalize to list of labels? *)
   Definition linker (ℓ : label) (Γ : list type) (τ : type) : ctx :=
@@ -32,15 +30,58 @@ Section linker.
     apply LamN_ctx_typed. repeat econstructor.
   Qed.
 
-
 End linker.
 
-(* Section dyn_emb. *)
+From main.prelude Require Import autosubst.
+From main.grad_lang Require Import labels.
+From main.maps Require Import grad_into_dyn.definition.
+From main.logrel Require Import definition lemmas.fun_grad_into_dyn.
+From main.dyn_lang Require Import definition contexts.
+From main.maps.linker.components Require Import lemmas agree.
 
-(*   Context {ν : label} {Hν : NeverOccurs ν}. *)
+Section lemmas.
 
-(*   Definition import (ℓ : label) (Γ : list type) (τ : type) (e : dexpr) : gexpr := *)
-(*      Wrap_g (Ascribe ℓ Unknown τ ⌜⌜e⌝⌝) *)
-(*        ((fun τ => Lam (Ascribe ℓ τ Unknown (Var 0))) <$> Γ). *)
+  Context {ν : label} {Hν : NeverOccurs ν}.
 
-(* End dyn_emb. *)
+  Lemma linker_compat' L ℓ (H : L ℓ ℓ) Γ τ :
+            ctx_rel_typed L
+              (trns_ctx $ linker ℓ Γ τ)
+              (trns_ctx $ linker ℓ Γ τ) (replicate (length Γ) Unknown ++ Γ) Unknown Γ τ.
+  Proof.
+    eapply ctx_rel_typed_weaken.
+    2: { apply fundamental_ctx. apply linker_typed. }
+    rewrite /linker.
+    intros l l' Hll'.
+    rewrite /InGradCtx /unary_conj in Hll'.
+    assert (Ha := AppWithList_ctx_wrap_ctx_vars_ascribe_up_lables ℓ Γ).
+    repeat rewrite labels_ctx_app in Hll'.
+    rewrite LamN_ctx_lables in Hll'. simpl in Hll'. destruct Hll' as [a b].
+    assert ((l ∈ ({[ℓ]} : listset label))). set_solver.
+    assert ((l' ∈ ({[ℓ]} : listset label))). set_solver.
+    by rewrite (elem_of_singleton_1 _ _ H0) (elem_of_singleton_1 _ _ H1).
+  Qed.
+
+  Lemma linker_compat L ℓ (H : L ℓ ℓ) Γ e e' (HCe : Closed_n (length Γ) e) (HCe' : Closed_n (length Γ) e') τ :
+    open_exprel_typed (replicate (length Γ) Unknown) L e e' Unknown →
+    open_exprel_typed Γ L (fill_ctx (trns_ctx (linker ℓ Γ τ)) e)
+                          (fill_ctx (trns_ctx (linker ℓ Γ τ)) e') τ.
+  Proof.
+    intros Hee'.
+    apply (linker_compat' L ℓ H Γ τ L (le_permissive_same L) e e').
+    apply open_exprel_typed_app_ctx; eauto; try by rewrite replicate_length.
+  Qed.
+
+  Lemma linker_superfluous_l L ℓ Γ e e' (HCe : Closed_n (length Γ) e) τ :
+    open_exprel_typed Γ L e e' τ →
+    open_exprel_typed Γ L (fill_ctx (trns_ctx (linker ℓ Γ τ)) e) e' τ.
+  Proof.
+    intro Hee'.
+    rewrite /linker. repeat rewrite trns_ctx_app.
+    rewrite AppWithList_ctx_agree LamN_ctx_agree /=.
+    rewrite wrap_ctx_vars_ascribe_up_agree /=.
+    repeat rewrite -fill_ctx_app /=.
+    rewrite fill_LamN_ctx fill_AppWithList_ctx.
+    apply open_exprel_superfluous_ctx_l; auto.
+  Qed.
+
+End lemmas.
