theories/prelude/lists.v
@@ -1,0 +1,26 @@
+From main Require Import prelude.imports.
+From stdpp Require Import list.
+
+Lemma Forall2_rev_ind {A B : Type} : ∀ (R : A → B → Prop) ( P : list A → list B → Prop ),
+  P [] []
+  → (∀ (x : A) (y : B) (l : list A) (l' : list B), R x y → Forall2 R l l' → P l l' → P (l ++ [x]) (l' ++ [y]))
+    → ∀ (l : list A) (l' : list B), Forall2 R l l' → P l l'.
+Proof.
+  intros R P HP0 HPS l.
+  induction l using rev_ind.
+  - intros l' HF.
+    assert (abs := Forall2_length _ _ _ HF). destruct l'; inversion abs. auto.
+  - intros l' HF.
+    destruct l' as [|x' l'] using rev_ind.
+    assert (abs := Forall2_length _ _ _ HF). rewrite app_length /= in abs. lia.
+    assert (H := Forall2_length _ _ _ HF). repeat rewrite app_length /= Nat.add_comm /= in H. inversion H.
+    edestruct (Forall2_app_inv _ l [x] l' [x'] H1 HF) as [a b].
+    apply HPS; auto. by inversion b; simplify_eq.
+Qed.
+
+Lemma Forall2_rev_ind' {A B : Type} {l : list A} {l' : list B} {R : A → B → Prop} :
+  Forall2 R l l' → ∀ ( P : list A → list B → Prop ),
+    P [] []
+    → (∀ (x : A) (y : B) (l : list A) (l' : list B), R x y → Forall2 R l l' → P l l' → P (l ++ [x]) (l' ++ [y]))
+      → P l l'.
+Proof. intros. eapply Forall2_rev_ind; eauto. Qed.
