theories/theorems/imported_wb_innocent.v
@@ -1,0 +1,67 @@
+From main.prelude Require Import imports autosubst.
+From main.maps Require Import
+  dyn_embedding.definition linker.definition grad_into_dyn.definition.
+From main.grad_lang Require Import definition types typing contexts labels.
+From main.dyn_lang Require Import definition contexts labels casts.
+From main.logrel Require Import definition adequacy.
+From main.logrel.lemmas Require Import fun_grad_into_dyn fun_dyn_embedding.
+
+Notation dexpr := dyn_lang.definition.expr.
+Notation gexpr := grad_lang.definition.expr.
+Notation gctx := grad_lang.contexts.ctx.
+Notation gfill_ctx := grad_lang.contexts.fill_ctx.
+
+Section dyn_emb.
+
+  Context {ν : label} {Hν : NeverOccurs ν}.
+  (* Definition irrelevant := Lbl 11. *)
+  (* Instance irrelevant : NeverOccurs (Lbl 11) := {}. *)
+
+  Definition Innocent Γ τ (e : gexpr) : Prop :=
+     ∀ (C : gctx) τ' (HC : typed_ctx C Γ τ [] τ'),
+     (∀ ℓ, rtc step ⌊ gfill_ctx C e ⌋ (Error ℓ) → ℓ ∈ (labels_ctx C)).
+
+  Definition WellBehaved Γ (e : dexpr) τ : Prop :=
+     open_exprel_typed Γ ∅ e e τ ∧ Closed_n (length Γ) e.
+
+  Definition import ℓ Γ τ (e : dexpr) : gexpr :=
+     gfill_ctx (linker ℓ Γ τ) ⌜⌜ e ⌝⌝.
+
+  Theorem importing_well_behaved_innocent Γ (e : dexpr) τ :
+    WellBehaved Γ e τ → ∀ ℓ, Innocent Γ τ (import ℓ Γ τ e).
+  Proof.
+    intros [Hee HCe] ℓ C τ' HC ℓ' H.
+    repeat rewrite trns_fill_ctx in H.
+    (* *)
+    assert (HC' := fundamental_ctx C _ _ _ _ HC).
+    assert (Hee' := fundamental_l _ _ HCe).
+    (* *)
+    assert (HR12 : RefineL (InGradCtx C ⊔ (unary_conj (eq ℓ)) ⊔ InDynExpr e)
+              (fill_ctx (trns_ctx C)
+                  (fill_ctx (trns_ctx (linker ℓ Γ τ)) ⌊ ⌜⌜ e ⌝⌝ ⌋))
+              (fill_ctx (trns_ctx C)
+                  (fill_ctx (trns_ctx (linker ℓ Γ τ)) e))).
+    { eapply logrel_adequacy. apply HC'.
+      { eapply le_permissive_trans'. apply compats.disj_le1. apply compats.disj_le1. }
+      apply linker_compat; auto.
+      { eapply le_permissive_trans'. apply compats.disj_le1. apply compats.disj_le2. rewrite /unary_conj. auto. }
+      by apply dyn_emb_trns_pres_closed_n.
+      eapply open_exprel_typed_weaken. apply Hee'. apply compats.disj_le2.
+    }
+    assert (HR23 : RefineL (InGradCtx C)
+              (fill_ctx (trns_ctx C)
+                  (fill_ctx (trns_ctx (linker ℓ Γ τ)) e))
+              (fill_ctx (trns_ctx C) e)).
+    { eapply logrel_adequacy. apply HC'. apply le_permissive_same.
+      apply linker_superfluous_l. auto.
+      eapply open_exprel_typed_weaken. apply Hee. intros l l' H'. by exfalso. }
+    assert (HR13 := (refineL_trans _ _ _ _ _ HR12 HR23)). clear HR12 HR23.
+    (* *)
+    destruct HR13 as [H1 H2]. specialize (H2 _ H).
+    destruct H2 as [l' (P & H')].
+    rewrite /comb_trans_lblrel /disj in P.
+    destruct P as (l2 & PP). rewrite /InGradCtx /diag /InDynExpr /InGradCtx in PP.
+    destruct PP. repeat destruct H0; try set_solver.
+  Qed.
+
+End dyn_emb.
